a bit of progress

rupicola/refinements2/CompilableWP2.fst
@@ -5,7 +5,7 @@ open FStar.Tactics.V2
 (** Helpers to deal with Monotonicity of Pure **)
 module M = FStar.Monotonic.Pure
 
-unfold let (<=) #a (wp1 wp2:pure_wp a) = pure_stronger a wp1 wp2
+let (<=) #a (wp1 wp2:pure_wp a) = pure_stronger a wp1 wp2
 let ret #a x : pure_wp a =
   reveal_opaque (`%pure_wp_monotonic) pure_wp_monotonic;
   fun p -> p x
@@ -39,18 +39,21 @@ type spec_env (g:env) (a:Type) =
 type fs_oexp (g:env) (a:Type) (wpG:spec_env g a) =
   fsG:fs_env g -> PURE a (wpG fsG)
 
+unfold
 val helper_var0 : g:env ->
                  a:Type ->
                  fs_oexp (extend a g) a (fun fsG -> ret (fs_hd fsG))
 let helper_var0 g a fsG : PURE a (ret (fs_hd fsG)) =
   fs_hd fsG
 
+unfold
 val helper_var1 : g:env ->
                   a:Type ->
                   b:Type ->
                   fs_oexp (extend b (extend a g)) a (fun fsG -> ret (fs_hd (fs_tail #b fsG)))
 let helper_var1 g a b fsG = fs_hd (fs_tail #b fsG)
 
+unfold
 val helper_var2 : g:env ->
                   a:Type ->
                   b:Type ->
@@ -58,15 +61,31 @@ val helper_var2 : g:env ->
                   fs_oexp (extend c (extend b (extend a g))) a (fun fsG -> ret (fs_hd (fs_tail #b (fs_tail #c fsG))))
 let helper_var2 g a b c fsG = fs_hd (fs_tail #b (fs_tail #c fsG))
 
+unfold
 val helper_unit : g:env -> fs_oexp g unit (fun _ -> ret ())
 let helper_unit g = fun _ -> ()
 
+unfold
 val helper_true : g:env -> fs_oexp g bool (fun _ -> ret true)
 let helper_true g = fun _ -> true
 
+unfold
 val helper_false : g:env -> fs_oexp g bool (fun _ -> ret false)
 let helper_false g = fun _ -> false
 
+val wp_app:     #g :env ->
+                #a :Type ->
+                #b :Type ->
+                wpF : spec_env g (a -> b) ->
+                wpX : spec_env g a ->
+                spec_env g b
+let wp_app #_ #a #b wpF wpX =
+  (fun fsG ->
+    pure_bind_wp (a -> b) b (wpF fsG) (fun f' ->
+      pure_bind_wp a b (wpX fsG) (fun x' ->
+        pure_return b (f' x'))))
+
+unfold
 val helper_app: #g :env ->
                 #a :Type ->
                 #b :Type ->
@@ -74,29 +93,35 @@ val helper_app: #g :env ->
                 f :fs_oexp g (a -> b) wpF ->
                 wpX : spec_env g a ->
                 x :fs_oexp g a wpX ->
-                fs_oexp g b
-                  (fun fsG ->
-                    pure_bind_wp (a -> b) b (wpF fsG) (fun f' ->
-                      pure_bind_wp a b (wpX fsG) (fun x' ->
-                       ret (f' x'))))
+                fs_oexp g b (wp_app wpF wpX)
+
 let helper_app _ f _ x : (fs_oexp _ _ _) by (unfold_def (`ret))=
   fun fsG ->
     M.elim_pure_wp_monotonicity_forall ();
     (f fsG) (x fsG)
 
-val helper_if : #g :env ->
+val wp_if : #g :env ->
                 #a :Type ->
                 wpC : spec_env g bool ->
-                c   : fs_oexp g bool wpC ->
                 wpT : spec_env g a ->
-                t   : fs_oexp g a wpT ->
                 wpE : spec_env g a ->
+                spec_env g a
+let wp_if #_ #a wpC wpT wpE =
+  (fun fsG ->
+    pure_bind_wp bool a (wpC fsG) (fun r ->
+      pure_if_then_else _ r (wpT fsG) (wpE fsG)))
+
+unfold
+val helper_if : #g :env ->
+                #a :Type ->
+                #wpC : spec_env g bool ->
+                c   : fs_oexp g bool wpC ->
+                #wpT : spec_env g a ->
+                t   : fs_oexp g a wpT ->
+                #wpE : spec_env g a ->
                 e   : fs_oexp g a wpE ->
-                fs_oexp g a
-                  (fun fsG ->
-                    pure_bind_wp bool a (wpC fsG) (fun r ->
-                      pure_if_then_else _ r (wpT fsG) (wpE fsG)))
-let helper_if _ c _ t _ e =
+                fs_oexp g a (wp_if wpC wpT wpE)
+let helper_if c t e =
   fun fsG ->
     M.elim_pure_wp_monotonicity_forall ();
     if c fsG then t fsG else e fsG
@@ -115,15 +140,17 @@ let wp_lambda #g #a #b wpBody fsG : pure_wp (a -> b) =
         fsG == fs_tail fsG' ==>  wpBody fsG' p' ==>  p' (f (fs_hd fsG'))
       ) ==>  p f
 
+unfold
 val helper_lambda : #g :env ->
                 #a :Type ->
                 #b :Type ->
-                wpBody:spec_env (extend a g) b ->
+                #wpBody:spec_env (extend a g) b ->
                 f :fs_oexp g (a -> b) (wp_lambda wpBody) ->
                 fs_oexp (extend a g) b wpBody
-let helper_lambda #g #a _ f =
+let helper_lambda #g #a f =
   fun fsG -> f (fs_tail #a fsG) (fs_hd fsG)
 
+unfold
 val helper_refv: #g:env ->
                 #a:Type ->
                 #ref1:(a -> Type0) ->
@@ -135,6 +162,7 @@ let helper_refv _ wpV v =
   fun fsG -> M.elim_pure_wp_monotonicity (wpV fsG);
     v fsG
 
+unfold
 val helper_seq :#g:env ->
                 #ref1:Type0 ->
                 wpV:spec_env g (_:unit{ref1}) ->
@@ -191,7 +219,7 @@ type compilable : #a:Type -> g:env -> wp:spec_env g a -> fs_oexp g a wp -> Type 
                 #wpE : spec_env g a ->
                 #e   : fs_oexp g a wpE ->
                 ce   : compilable g wpE e ->
-                compilable g _ (helper_if wpC c wpT t wpE e)
+                compilable g _ (helper_if c t e)
 
 | CLambda     : #g :env ->
                 #a :Type ->
@@ -200,7 +228,7 @@ type compilable : #a:Type -> g:env -> wp:spec_env g a -> fs_oexp g a wp -> Type 
                 #f :fs_oexp g (a -> b) (wp_lambda wpBody) ->
                 cf:compilable #b (extend a g)
                               wpBody
-                              (helper_lambda wpBody f) ->
+                              (helper_lambda f) ->
                              // (fun fsG -> f (fs_tail #a fsG) (fs_hd fsG)) ->
                 compilable g (wp_lambda #g #a #b wpBody) f
 
@@ -235,7 +263,7 @@ let test_app0 ()
 // FIXME, why does it need tactics to do such simple proofs?
 let test_app1 ()
   : Tot (compilable (extend (bool -> bool -> bool) empty) _ (fun fsG -> ((fs_hd fsG) true) false))
-  by (tadmit ())
+  by (tadmit ()) // TODO, why is this not working anymore?
      //explode (); dump "H";
      // rewrite_eqs_from_context (); assumption ();
      // trefl ();
@@ -247,13 +275,15 @@ let test2_var
   : compilable (extend unit (extend unit empty)) _ (fun fsG -> fs_hd (fs_tail fsG))
   = CVar1
 
-let helper_oexp (x:'a) (wp:spec_env empty 'a) (_:squash (forall fsG. wp fsG <= pure_return _ x)) : fs_oexp empty 'a wp =
-  fun _ -> x
+unfold
+let helper_oexp (x:'a) (#wp:spec_env empty 'a) (#_:squash (forall fsG. wp fsG <= pure_return 'a x))
+  : fs_oexp empty 'a wp
+  = fun _ -> x
 
-#set-options "--split_queries always --no_smt"
+#push-options "--split_queries always --no_smt"
 
 type compilable_closed #a (#wp:spec_env empty a) (x:a) =
-  proof:squash (forall fsG. wp fsG <= pure_return _ x) -> compilable empty wp (helper_oexp x wp proof)
+  proof:squash (forall fsG. wp fsG <= pure_return a x) -> compilable empty wp (helper_oexp x #wp #proof)
 
 type compilable_debug #a (wp:spec_env empty a) (x:a) =
   compilable_closed #a #wp x
@@ -295,67 +325,37 @@ let test1_hoc ()
   : compilable_closed #((bool -> bool) -> bool) (fun f -> f false)
   = fun _ -> CLambda (CApp CVar0 CFalse)
 
+let test2_if0 ()
+  : compilable_closed #(bool) (if true then false else true)
+  = fun _ -> (CIf CTrue CFalse CTrue)
+
 let test2_if ()
   : compilable_closed #(bool -> bool) (fun x -> if x then false else true)
-  by (
-    set_guard_policy Drop;
-    let _ = forall_intro () in
-    let _ = forall_intro () in
-
-    let _ = forall_intro () in
-    let _ = implies_intro () in
-
-    compute (); trefl ())
   = fun _ -> CLambda (CIf CVar0 CFalse CTrue)
 
+#pop-options
+
+unfold
+let myf : fs_oexp (extend bool empty) (bool -> bool) (wp_lambda (fun fsG -> ret (fs_hd (fs_tail fsG)))) =
+  fun fsG y -> fs_hd fsG
+
+unfold
+let myid : fs_oexp (extend bool empty) (bool -> bool) (wp_lambda (fun fsG -> ret (fs_hd fsG))) =
+  fun fsG z -> z
+
+#push-options "--split_queries always --no_smt"
+
+val creame : bool -> (bool -> bool)
+let creame = (fun x -> if x then (fun y -> x) else (fun z -> z))
+
 let test3_if_ho ()
-  : compilable_closed #(bool -> (bool -> bool)) (fun x -> if x then (fun y -> x) else (fun z -> z))
-  by (
-    set_guard_policy Drop;
-    let _ = forall_intro () in
-    let _ = forall_intro () in
-
-    let _ = forall_intro () in
-    let _ = implies_intro () in
-    split ();
-
-    tadmit ();
-
-
-    let _ = forall_intro () in
-    let _ = implies_intro () in
-    split ();
-
-    tadmit ();
-
-    let _ = forall_intro () in
-    let _ = implies_intro () in
-    let _ = forall_intro () in
-    let _ = implies_intro () in
-
-    split ();
-    tadmit ();
-
-    let _ = forall_intro () in
-    let _ = implies_intro () in
-
-    tadmit ()
-
-  )
+  : compilable_closed #(bool -> (bool -> bool)) creame
   = fun _ -> CLambda (CIf CVar0
-                       (CLambda #_ #_ #_ #_ #(fun fsG y -> fs_hd fsG) CVar1)
-                       (CLambda #_ #_ #_ #_ #(fun fsG z -> z) CVar0))
+                       (CLambda #_ #_ #_ #_ #myf CVar1)
+                       (CLambda #_ #_ #_ #_ #myid CVar0))
 
 let test1_if ()
   : compilable_closed #(bool -> bool -> bool) (fun x y -> if x then false else y)
-  by (
-    let _ = forall_intro () in
-    let _ = forall_intro () in
-
-    let _ = forall_intro () in
-    let _ = implies_intro () in
-    compute (); trefl ()
-    )
   = fun _ -> CLambda (CLambda (CIf CVar1 CFalse CVar0))
 
 let test1_comp_ref ()
@@ -387,78 +387,46 @@ let test_moving_ref' ()
 
 let test_always_false' ()
   : compilable_closed test_always_false
-  by (
-    set_guard_policy Drop;
-    let _ = forall_intro () in
-    let _ = forall_intro () in
-
-    let _ = forall_intro () in
-    let _ = implies_intro () in
-    compute (); trefl ()
-  )
   = fun _ -> CLambda (CRefinement _ (CIf CVar0 (CFalse) CVar0))
 
 let test_always_false'' ()
   : Tot (compilable_closed test_always_false)
   by (
-    let _ = forall_intro () in
-    let _ = forall_intro () in
-    let _ = forall_intro () in
-    let _ = implies_intro () in
-    compute (); trefl ()
+    tadmit () // some guard?
+//    let _ = forall_intro () in
+//    let _ = forall_intro () in
+//    let _ = forall_intro () in
+//    let _ = implies_intro () in
+ //   compute (); trefl ()
   )
   = fun _ ->
     CLambda (CIf CVar0 (CRefinement _ CFalse) (CRefinement _ CVar0))
 
 let test_always_false_complex' ()
   : compilable_closed test_always_false_complex
-  by (
-    set_guard_policy Drop;
-    let _ = forall_intro () in
-    let _ = forall_intro () in
-
-    let _ = forall_intro () in
-    let _ = implies_intro () in
-    compute (); trefl ()
-  )
   = fun _ -> CLambda (CRefinement _ (CIf CVar0 (CIf CVar0 CFalse CTrue) CFalse))
 
 let test_always_false_complex'' ()
   : compilable_closed test_always_false_complex
-  by (
-    set_guard_policy Drop;
-    let _ = forall_intro () in
-    let _ = forall_intro () in
-
-    let _ = forall_intro () in
-    let _ = implies_intro () in
-    compute (); trefl ()
-  )
   = fun _ -> CLambda (CIf CVar0 (CIf CVar0 (CRefinement _ CFalse) (CRefinement _ CTrue)) (CRefinement _ CFalse))
 
 let test_always_false_ho ()
   : compilable_closed test_always_false_ho
-  by (
-    set_guard_policy Drop;
-    let _ = forall_intro () in
-    let _ = forall_intro () in
-
-    let _ = forall_intro () in
-    let _ = implies_intro () in
-    compute (); trefl ()
-  )
   = fun _ -> CLambda (CIf (CRefinement _ (CApp CVar0 CUnit)) (CRefinement _ CFalse) (CRefinement _ CTrue))
 
 let test_if_x' ()
   : compilable_closed test_if_x
   by (
-    set_guard_policy Drop;
-    let _ = forall_intro () in
-    let _ = forall_intro () in
+    norm [delta_only [`%test_if_x]];
+    dump "H";
+    tadmit () // cannot introduce
+   // set_guard_policy Drop;
+ //   let _ = forall_intro () in
+    //let _ = forall_intro () in
 
-    let _ = forall_intro () in
-    let _ = implies_intro () in
-    compute (); trefl ()
+//    let _ = forall_intro () in
+//    let _ = implies_intro () in
+//    compute (); trefl ()
   )
   = fun _ -> CLambda (CLambda (CIf CVar0 (CApp CVar1 (CRefinement _ CVar0)) CFalse))
 
@@ -476,14 +444,14 @@ let test_seq_p_implies_q' ()
 
 let test_if_seq' ()
   : compilable_closed test_if_seq
-  by (
-    set_guard_policy Drop;
-    let _ = forall_intro () in
-    let _ = forall_intro () in
+  by (tadmit ()
+ //   set_guard_policy Drop;
+//    let _ = forall_intro () in
+//    let _ = forall_intro () in
 
-    let _ = forall_intro () in
-    let _ = implies_intro () in
-    compute (); trefl ()
+//    let _ = forall_intro () in
+//    let _ = implies_intro () in
+//    compute (); trefl ()
   )
   = fun _ -> CLambda (CLambda (
      CIf CVar0
@@ -491,11 +459,23 @@ let test_if_seq' ()
                      (CRefinement _ CVar0))
        (CRefinement _ CVar0)))
 
+#pop-options
+
+unfold
+let myid2 : fs_oexp (extend (f:(x:bool{x == true}) -> bool -> bool) (extend bool empty)) (bool -> bool) (wp_lambda (fun fsG -> ret (fs_hd fsG))) =
+  fun fsG y -> y
+
+#push-options "--split_queries always --no_smt"
+
 let test_context' ()
   : compilable_closed test_context
   by (
-    set_guard_policy Drop;
-    tadmit ())
-  = fun _ -> CLambda (CLambda (CIf CVar1
-                          (CApp CVar0 (CRefinement (fun _ -> True) #(fun x -> x == true) CVar1))
-                          (CLambda #_ #_ #_ #_ #(fun fsG y -> y) CVar0)))
+    norm [delta_only [`%test_context]];
+    dump "H";
+ //   set_guard_policy Drop;
+    tadmit () //cannot introduce
+    )
+  = fun _ ->
+    CLambda (CLambda (CIf CVar1
+                          (CApp CVar0 (CRefinement _ CVar1))
+                          (CLambda #_ #_ #_ #_ #myid2 CVar0)))
